compute_degree with reduce_coeff

src/tactic/compute_degree.lean
@@ -26,9 +26,39 @@ See the doc-string for more details.
 We start with a goal of the form `f.(nat_)degree ≤ d`.  Recurse into `f` breaking apart sums,
 products and powers.  Take care of numerals, `C a, X (^ n), monomial a n` separately. -/
 
+namespace polynomial
+open_locale polynomial
+
+variables {R : Type*}
+
+section semiring
+variables [semiring R] {f g : R[X]} {d e n : ℕ}
+
+lemma coeff_bit1_zero (P : R[X]) :
+  (bit1 P).coeff 0 = bit1 (P.coeff 0) :=
+by simp only [bit1, bit0, coeff_add, coeff_one_zero, pi.add_apply, pi.one_apply]
+
+/-  This lemma is useful to expose the right hypotheses for `tactic.interactive.compute_degree`. -/
+lemma coeff_mul_of_nat_degree_le' (de : d + e = n) (df : f.nat_degree ≤ d) (eg : g.nat_degree ≤ e) :
+  (f * g).coeff n = f.coeff d * g.coeff e :=
+by rwa [← de, coeff_mul_of_nat_degree_le df eg]
+
+/-  This lemma is useful to expose the right hypotheses for `tactic.interactive.compute_degree`. -/
+lemma coeff_pow_of_nat_degree_le' (de : d * e = n) (df : f.nat_degree ≤ d) :
+  (f ^ e).coeff n = (f.coeff d) ^ e :=
+by rwa [← de, coeff_pow_of_nat_degree_le]
+
+lemma coeff_monomial_self {a : R} : coeff (monomial n a) n = a :=
+coeff_monomial.trans $ if_pos rfl
+
+end semiring
+
+end polynomial
+
 namespace tactic
-namespace compute_degree
+
 open expr polynomial
+namespace compute_degree
 
 /--  `guess_degree e` assumes that `e` is an expression in a polynomial ring, and makes an attempt
 at guessing the `nat_degree` of `e`.  Heuristics for `guess_degree`:
@@ -65,8 +95,35 @@ meta def guess_degree : expr → tactic expr
                                 pe ← to_expr ``(@nat_degree %%R %%inst) tt ff,
                                 pure $ expr.mk_app pe [e]
 
-/-- `resolve_sum_step` assumes that the current goal is of the form `f.nat_degree ≤ d`, failing
-otherwise.  It tries to make progress on the goal by progressing into `f` if `f` is
+/--  `guess_degree'` is very similar to `guess_degree`, except that it returns a `tactic ℕ`,
+instead of a `tactic expr`.  The main difference between the two is their dealing of non-closed
+natural numbers.  The difference allows `compute_degree_le` to work in *some* situations involving
+non-closed exponents.  -/
+meta def guess_degree' : expr → tactic ℕ
+| `(has_zero.zero)           := pure 0
+| `(has_one.one)             := pure 0
+| `(- %%f)                   := guess_degree' f
+| (app `(⇑C) x)              := pure 0
+| `(X)                       := pure 1
+| `(bit0 %%a)                := guess_degree' a
+| `(bit1 %%a)                := guess_degree' a
+| `(%%a + %%b)               := do [da, db] ← [a, b].mmap guess_degree',
+                                if da ≤ db then return db else return da
+| `(%%a - %%b)               := do [da, db] ← [a, b].mmap guess_degree',
+                                if da ≤ db then return db else return da
+| `(%%a * %%b)               := do [da, db] ← [a, b].mmap guess_degree',
+                                pure $ da + db
+| `(%%a ^ %%b)               := do da ← guess_degree' a,
+                                db ← eval_expr' ℕ b <|> pure 0,
+                                pure $ da * db
+| (app `(⇑(monomial %%n)) x) := eval_expr' ℕ n <|> pure 0
+| e                          := pure 0
+
+/-- `resolve_sum_step e` takes the type of the current goal `e` as input.
+It tries to make progress on the goal `e` by reducing it to subgoals.
+It assumes that `e` is of the form `f.nat_degree ≤ d`, failing otherwise.
+
+`resolve_sum_step` progresses into `f` if `f` is
 * a sum, difference, opposite, product, or a power;
 * a monomial;
 * `C a`;
@@ -75,35 +132,36 @@ otherwise.  It tries to make progress on the goal by progressing into `f` if `f`
 The side-goals produced by `resolve_sum_step` are either again of the same shape `f'.nat_degree ≤ d`
 or of the form `m ≤ n`, where `m n : ℕ`.
 
-If `d` is less than `guess_degree f`, this tactic will create unsolvable goals.
+If `d` is less than `guess_degree' f`, this tactic will create unsolvable goals.
 -/
-meta def resolve_sum_step : tactic unit := do
-t ← target >>= instantiate_mvars,
-`(nat_degree %%tl ≤ %%tr) ← whnf t reducible | fail!("Goal is not of the form `f.nat_degree ≤ d`"),
-match tl with
-| `(%%tl1 + %%tl2) := refine ``((nat_degree_add_le_iff_left _ _ _).mpr _)
-| `(%%tl1 - %%tl2) := refine ``((nat_degree_sub_le_iff_left _).mpr _)
-| `(%%tl1 * %%tl2) := do [d1, d2] ← [tl1, tl2].mmap guess_degree,
-  refine ``(nat_degree_mul_le.trans $ (add_le_add _ _).trans (_ : %%d1 + %%d2 ≤ %%tr))
-| `(- %%f)         := refine ``((nat_degree_neg _).le.trans _)
-| `(X ^ %%n)       := refine ``((nat_degree_X_pow_le %%n).trans _)
-| (app `(⇑(@monomial %%R %%inst %%n)) x) := refine ``((nat_degree_monomial_le %%x).trans _)
-| (app `(⇑C) x)    := refine ``((nat_degree_C %%x).le.trans (nat.zero_le %%tr))
-| `(X)             := refine ``(nat_degree_X_le.trans _)
-| `(has_zero.zero) := refine ``(nat_degree_zero.le.trans (nat.zero_le _))
-| `(has_one.one)   := refine ``(nat_degree_one.le.trans (nat.zero_le _))
-| `(bit0 %%a)      := refine ``((nat_degree_bit0 %%a).trans _)
-| `(bit1 %%a)      := refine ``((nat_degree_bit1 %%a).trans _)
-| `(%%tl1 ^ %%n)   := do
-    refine ``(nat_degree_pow_le.trans _),
-    refine ``(dite (%%n = 0) (λ (n0 : %%n = 0), (by simp only [n0, zero_mul, zero_le])) _),
-    n0 ← get_unused_name "n0" >>= intro,
-    refine ``((mul_comm _ _).le.trans ((nat.le_div_iff_mul_le' (nat.pos_of_ne_zero %%n0)).mp _)),
-    lem1 ← to_expr ``(nat.mul_div_cancel _ (nat.pos_of_ne_zero %%n0)) tt ff,
-    lem2 ← to_expr ``(nat.div_self (nat.pos_of_ne_zero %%n0)) tt ff,
-    focus1 (refine ``((%%n0 rfl).elim) <|> rewrite_target lem1 <|> rewrite_target lem2) <|> skip
-| e                := fail!"'{e}' is not supported"
-end
+meta def resolve_sum_step : expr → tactic unit
+| `(nat_degree %%tl ≤ %%tr) := match tl with
+  | `(%%tl1 + %%tl2) := refine ``((nat_degree_add_le_iff_left _ _ _).mpr _)
+  | `(%%tl1 - %%tl2) := refine ``((nat_degree_sub_le_iff_left _).mpr _)
+  | `(%%tl1 * %%tl2) := do [d1, d2] ← [tl1, tl2].mmap guess_degree,
+    refine ``(nat_degree_mul_le.trans $ (add_le_add _ _).trans (_ : %%d1 + %%d2 ≤ %%tr))
+  | `(- %%f)         := refine ``((nat_degree_neg _).le.trans _)
+  | `(X ^ %%n)       := refine ``((nat_degree_X_pow_le %%n).trans _)
+  | (app `(⇑(@monomial %%R %%inst %%n)) x) := refine ``((nat_degree_monomial_le %%x).trans _)
+  | (app `(⇑C) x)    := refine ``((nat_degree_C %%x).le.trans (nat.zero_le %%tr))
+  | `(X)             := refine ``(nat_degree_X_le.trans _)
+  | `(has_zero.zero) := refine ``(nat_degree_zero.le.trans (nat.zero_le _))
+  | `(has_one.one)   := refine ``(nat_degree_one.le.trans (nat.zero_le _))
+  | `(bit0 %%a)      := refine ``((nat_degree_bit0 %%a).trans _)
+  | `(bit1 %%a)      := refine ``((nat_degree_bit1 %%a).trans _)
+  | `(%%tl1 ^ %%n)   := do
+      refine ``(nat_degree_pow_le.trans _),
+      refine ``(dite (%%n = 0) (λ (n0 : %%n = 0), (by simp only [n0, zero_mul, zero_le])) _),
+      n0 ← get_unused_name "n0" >>= intro,
+      refine ``((mul_comm _ _).le.trans ((nat.le_div_iff_mul_le' (nat.pos_of_ne_zero %%n0)).mp _)),
+      focus1 (refine ``((%%n0 rfl).elim) <|>
+        to_expr ``(nat.mul_div_cancel _ (nat.pos_of_ne_zero %%n0)) tt ff >>= rewrite_target <|>
+        to_expr ``(nat.div_self (nat.pos_of_ne_zero %%n0)) tt ff >>= rewrite_target) <|>
+      skip
+  | e                := fail!"'{e}' is not supported"
+  end
+| e := fail!("'resolve_sum_step' was called on\n" ++
+  "{e}\nbut it expects `f.nat_degree ≤ d`")
 
 /--  `norm_assum` simply tries `norm_num` and `assumption`.
 It is used to try to discharge as many as possible of the side-goals of `compute_degree_le`.
@@ -127,23 +185,92 @@ meta def eval_guessing (n : ℕ) : expr → tactic ℕ
 | `(max %%a %%b) := max <$> eval_guessing a <*> eval_guessing b
 | e              := eval_expr' ℕ e <|> pure n
 
-/--  A general description of `compute_degree_le_aux` is in the doc-string of `compute_degree`.
-The difference between the two is that `compute_degree_le_aux` makes no effort to close side-goals,
-nor fails if the goal does not change. -/
-meta def compute_degree_le_aux : tactic unit := do
-try $ refine ``(degree_le_nat_degree.trans (with_bot.coe_le_coe.mpr _)),
-`(nat_degree %%tl ≤ %%tr) ← target |
-  fail "Goal is not of the form\n`f.nat_degree ≤ d` or `f.degree ≤ d`",
-expected_deg ← guess_degree tl >>= eval_guessing 0,
-deg_bound ← eval_expr' ℕ tr <|> pure expected_deg,
-if deg_bound < expected_deg
-then fail sformat!"the given polynomial has a term of expected degree\nat least '{expected_deg}'"
-else repeat $ resolve_sum_step
+/--  These are the cases in which an available lemma computes the degree.
+`single_term_suggestions` returns a pair `(e1, e2)`, where `e1` pretty-prints to something
+suitable for a "Try this:", while `e2` is an expression that unifies with the target. -/
+meta def single_term_suggestions : tactic (expr × (expr ff)) :=
+do
+  t ← target,
+  [ ``(polynomial.nat_degree_X_pow _),
+    ``(polynomial.nat_degree_C _),
+    ``(polynomial.nat_degree_X),
+    ``(polynomial.nat_degree_C_mul_X_pow _ _ ‹_›),
+    ``(polynomial.nat_degree_C_mul_X _ ‹_›) ].mfirst
+    (λ st, do
+      na ← to_expr st tt ff,
+      infer_type na >>= unify t >> return (replace_mvars na, st))
+
+/--
+`get_lead_coeff c e` assumes that `c` is an `instance_cache` of a `(semi_)ring R` and that `e`
+is an expression representing a polynomial with coefficients in the type `R`.  It returns an
+expression representing the "visible leading coefficient" of `e`.  This means that it guesses the
+degree of each term and simply discards the terms whose guessed degree is smaller than the top
+degree.
+
+It is important that `get_lead_coeff` does not do any other simplifications of the expression.
+Indeed, `resolve_coeff` starts with the equality between `coeff e <top_degree of e>` and
+`get_lead_coeff c e` and peels off one by one the operations that make up the expression of
+`get_lead_coeff c e`.  Thus, `get_lead_coeff` guides the simplifications in the coefficients.
+In particular, there is some duplication of code with which `norm_num` could deal, but, following
+the current strategy, we are able to reach places where `norm_num` would not reach: most notably,
+`resolve_coeff` deals with degrees of products and of powers.
+
+The implementation of `get_lead_coeff` is a straightforward match on the elementary operations
+that can be performed on a polynomial.
+-/
+meta def get_lead_coeff (c : instance_cache) : expr → tactic (instance_cache × expr)
+| (app `(⇑C) a) := pure (c, a)
+| (app `(⇑(monomial %%n)) x) := pure (c, x)
+| `(@has_one.one (@polynomial %%R %%_) %%_) := c.mk_app ``has_one.one []
+| `(@has_zero.zero (@polynomial %%R %%_) %%_) := c.mk_app ``has_zero.zero []
+| `(X) := c.mk_app ``has_one.one []
+| `(X ^ %%n) := c.mk_app ``has_one.one []
+| `(bit0 %%a) := do
+  (c, ta) ← get_lead_coeff a,
+  c.mk_bit0 ta
+| `(bit1 %%a) := do
+  (c, ta) ← get_lead_coeff a,
+  c.mk_bit1 ta
+| `(%%a + %%b) := do
+  [da, db] ← [a,b].mmap guess_degree',
+  if da ≠ db then
+    if da < db then
+      get_lead_coeff b
+    else
+      get_lead_coeff a
+  else do
+    [(c1, ta), (c2, tb)] ← [a, b].mmap $ get_lead_coeff,
+    c1.mk_app ``has_add.add [ta, tb]
+| `(%%a - %%b) := do
+  [da, db] ← [a,b].mmap guess_degree',
+  if da ≠ db then
+    if da < db then do
+      (c, tb) ← get_lead_coeff b,
+      c.mk_app ``has_neg.neg [tb]
+    else
+      get_lead_coeff a
+  else do
+    [(c1, ta), (c2, tb)] ← [a, b].mmap get_lead_coeff,
+    c1.mk_app ``has_sub.sub [ta, tb]
+| `(%%a * %%b) := do
+  [(c1, ta), (c2, tb)] ← [a, b].mmap get_lead_coeff,
+  c1.mk_app ``has_mul.mul [ta, tb]
+| `(%%a ^ %%n) := do
+  (c, ta) ← get_lead_coeff a,
+  op ← to_expr ``(has_pow.pow : %%c.α → ℕ → %%c.α),
+  return $ (c, op.mk_app [ta, n])
+| `(- %%a) := do
+  (c, ta) ← get_lead_coeff a,
+  c.mk_app ``has_neg.neg [ta]
+| e := do
+  deg ← guess_degree e,
+  op ← to_expr ``(coeff : polynomial %%c.α → ℕ → %%c.α),
+  return $ (c, op.mk_app [e, deg])
 
 end compute_degree
 
 namespace interactive
-open compute_degree polynomial
+open compute_degree
 
 /--  `compute_degree_le` tries to solve a goal of the form `f.nat_degree ≤ d` or `f.degree ≤ d`,
 where `f : R[X]` and `d : ℕ` or `d : with_bot ℕ`.
@@ -172,8 +299,234 @@ by compute_degree_le
 ```
 -/
 meta def compute_degree_le : tactic unit :=
-focus1 $ do check_target_changes compute_degree_le_aux,
+focus1 $ do
+  t ← target,
+  try $ refine ``(degree_le_nat_degree.trans (with_bot.coe_le_coe.mpr _)),
+  `(nat_degree %%tl ≤ %%tr) ← target |
+    fail "Goal is not of the form\n`f.nat_degree ≤ d` or `f.degree ≤ d`",
+  expected_deg ← guess_degree' tl,
+  deg_bound ← eval_expr' ℕ tr <|> pure expected_deg,
+  if deg_bound < expected_deg
+  then fail sformat!"the given polynomial has a term of expected degree\nat least '{expected_deg}'"
+  else
+    repeat $ target >>= instantiate_mvars >>= resolve_sum_step,
+  (do gs ← get_goals >>= list.mmap infer_type,
+    success_if_fail $ gs.mfirst $ unify t) <|> fail "Goal did not change",
   try $ any_goals' norm_assum
+
+end interactive
+
+namespace compute_degree
+open interactive
+/--
+`resolve_coeff` assumes that the goal has the form `f.coeff n = x`.  It is important that `x`
+is the result of applying `get_lead_coeff` to `f`!  Indeed, `resolve_coeff` reads through the
+expression making up `f` and matches each step with what `get_lead_coeff` would do in the current
+situation.  This means that all the side-goals that `resolve_coeff` leaves are always of the same
+shape `f'.coeff n' = get_lead_coeff c f'`.
+
+In some sense, this views `coeff _ <visible_top_degree>` as a "monad" converting between
+`R[X]` and `R`.  `resolve_coeff` performs the operations building `f` across the monad.
+-/
+meta def resolve_coeff : tactic unit :=
+focus1 $ do
+  tg ← target >>= instantiate_mvars,
+  `(coeff %%f %%n = _) ← pure tg | fail!"{tg} is not of the form\n`f.coeff n = x`",
+  match f with
+  | `(@has_one.one %%RX %%_)            := refine ``(coeff_one_zero)
+  | (app `(⇑C) _)                       := refine ``(coeff_C_zero)
+  | (app `(⇑(@monomial %%R %%_ %%n)) x) := refine ``(coeff_monomial_self)
+  | `(X)                                := refine ``(coeff_X_one)
+  | `(X ^ %%n)                          := refine ``(coeff_X_pow_self %%n)
+  | `(bit0 %%a) := do
+    refine ``((coeff_bit0 _ _).trans _),
+    refine ``(congr_arg bit0 _),
+    reflexivity <|> resolve_coeff
+  | `(bit1 %%a) := do
+    refine ``((coeff_bit1_zero _).trans _),
+    refine ``(congr_arg bit1 _),
+    reflexivity <|> resolve_coeff
+  | `(%%a + %%b) := do
+    [da, db] ← [a,b].mmap guess_degree',
+    (if da ≠ db then do
+      if da < db then refine ``((coeff_add_eq_right_of_lt (nat.lt_succ_iff.mpr _)).trans _)
+      else refine ``((coeff_add_eq_left_of_lt (nat.lt_succ_iff.mpr _)).trans _),
+      compute_degree_le
+    else refine ``((coeff_add _ _ _).trans _);
+    congr' (some 1));
+    resolve_coeff
+  | `(%%a - %%b) := do
+    [da, db] ← [a,b].mmap guess_degree',
+    (if da ≠ db then do
+      if da < db then refine ``((coeff_sub_eq_neg_right_of_lt (nat.lt_succ_iff.mpr _)).trans
+        (neg_inj.mpr _))
+      else refine ``((coeff_sub_eq_left_of_lt (nat.lt_succ_iff.mpr _)).trans _),
+      compute_degree_le
+    else refine ``((coeff_sub _ _ _).trans _) >> congr' (some 1));
+    resolve_coeff
+  | `(%%a * %%b) := do
+    [da, db] ← [a,b].mmap guess_degree,
+    refine ``((coeff_mul_of_nat_degree_le' (by norm_num : %%da + %%db = %%n) _ _).trans _),
+    iterate_at_most' 2 compute_degree_le,
+    try $ congr' (some 1);
+    resolve_coeff
+  | `(%%a ^ %%ex) := do
+    da ← guess_degree a,
+    refine ``((coeff_pow_of_nat_degree_le' (by norm_num : %%da * %%ex = _) _).trans _),
+    compute_degree_le,
+    try $ congr' (some 1);
+    resolve_coeff
+  | `(- %%a) := do
+    refine ``((coeff_neg _ _).trans (neg_inj.mpr _)),
+    resolve_coeff
+  | e := skip
+  end
+
+setup_tactic_parser
+/--  `poly_and_deg_to_equation de f deg (with na)?` takes as input
+* an "option format" to distinguish whether it was called by `simp_coeff` (`none`) or
+  `reduce coeff` (`some fmt`),
+* an expression `f` representing a polynomial,
+* an expression `deg` representing an natural number and
+* an optional `with h` argument to assign a name to the side-goal that the tactic produces.
+It returns
+* a term `h` of type `f.coeff deg = lc`, where `lc` is the leading coefficient of `f`, computed by
+  `get_lead_coeff`;
+* as a side-goal to show the equality ``f.coeff deg = lc`.
+The input `de` is only used for reporting errors. -/
+meta def poly_and_deg_to_equation (de : option format) (f deg : expr) (na : parse with_ident_list) :
+  tactic expr :=
+do
+  `(@polynomial %%R %%_) ← infer_type f,
+  c ← mk_instance_cache R,
+  (c, lc) ← get_lead_coeff c f,
+  ide ← match na with
+    | []      := pure `c_c
+    | [a]     := pure a
+    | (a::as) := do pa ← pp a,
+      match de with
+      | some pfp := fail format!"Try this: reduce_coeff {pfp} with {pa}"
+      | none     := fail format!"Try this: simp_coeff with {pa}"
+      end
+    end,
+  nn ← get_unused_name ide,
+  cf ← to_expr ``(coeff : polynomial %%R → ℕ → %%R),
+  co_eq_co ← mk_app `eq [cf.mk_app [f, deg], lc],
+  assert nn co_eq_co
+
+end compute_degree
+
+namespace interactive
+open compute_degree
+
+section parsing
+setup_tactic_parser
+
+/--
+`simp_coeff (with h)?` assumes that the target is either of the form `f.coeff n = x` or of the form
+`f.coeff n ≠ x`.  It then proceeds to simplify `f.coeff n` recurring to the pair
+`get_lead_coeff/resolve_coeff` to scan the expression of `f` and producing a hopefully simpler
+expression.  After this, it calls on `simp only [a few lemmas]` and `norm_num` to simplify further.
+If the optional `with h` argument is given, then `h` is the name that `simp_coeff` assigns to
+possible side-goals.
+-/
+meta def simp_coeff (na : parse with_ident_list) : tactic unit :=
+do t ← target >>= instantiate_mvars,
+  (t_is_eq, f, m) ← match t with
+    | `(coeff %%f %%m = _) := return (tt, f, m)
+    | `(coeff %%f %%m ≠ _) := return (ff, f, m)
+    | _ := fail "Goal is not of the form `f.coeff n = x` or `f.coeff n ≠ x`"
+    end,
+  d_nat ← guess_degree' f,
+  m_nat ← eval_expr' ℕ m,
+  guard (d_nat = m_nat) <|> fail!(
+  "`simp_coeff` checks that the expected degree is equal to the degree appearing in `coeff`\n" ++
+  "the expected degree is `{d_nat}`, but you are asking about the coefficient of degree `{m_nat}`"),
+  c_c ← poly_and_deg_to_equation none f m na,
+  interactive.swap,
+  if t_is_eq then refine ``(eq.trans %%c_c _) else refine ``(ne_of_eq_of_ne %%c_c _),
+  try $ tactic.clear c_c,
+  refine ``(one_ne_zero) <|> interactive.swap,
+  resolve_coeff
+
+/--
+`reduce_coeff f (with h)?` takes a polynomial `f` as an input and produces a hypothesis of the form
+`c_c : f.coeff n = <simplified expression>`, where the simplified expression is obtained via the
+`get_lead_coeff/resolve_coeff` pair.
+If the optional `with h` argument is given, then `h` is the name that `reduce_coeff` assigns to
+possible side-goals.
+-/
+meta def reduce_coeff (fp : parse texpr) (na : parse with_ident_list) : tactic unit :=
+do
+  f ← to_expr ``(%%fp) tt ff,
+  exp_deg ← guess_degree' f,
+  pfp ← to_expr fp >>= pp,
+  poly_and_deg_to_equation pfp f `(exp_deg) na,
+  resolve_coeff
+
+/--  `compute_degree` tries to close goals of the form `f.(nat_)degree = d`.  It converts the
+goal to showing that
+* the degree is at most `d`, calling `compute_degree_le` to solve this case;
+* the coefficient of degree `d` is non-zero, calling `simp_coeff` to simplify this goal.
+
+Unless the polynomial is particularly complicated, `compute_degree` either succeeds of leaves
+a simpler goal to prove.  Continue reading for a discussion of what are the current
+limitations to the tactic.
+
+`compute_degree` scans the polynomial `f` and computes the largest degree `n` that it sees.
+It then assumes that this degree `n` equals the expected degree `d`, failing otherwise.
+
+In practice, this means that if the goal is `nat_degree (X - X + 1 : ℤ[X]) = 0`, then
+`compute_degree` gives an error, since there are terms of degree `1` in the expression
+(the cancelling pair `X, -X`) and the tactic expects `1` to be the degree.  Note that this is not
+an issue if the cancellation arises in terms of degrees smaller than the maximum:
+```lean
+example : nat_degree (X ^ 2 + X - X : ℤ[X]) = 2 := by compute_degree
+```
+works. -/
+meta def compute_degree (single : parse (tk "!" )?) : tactic unit :=
+focus $ do
+  t ← target >>= (λ f, whnf f reducible),
+  match t with
+  -- the `degree` match implicitly assumes that the `nat_degree` is strictly positive
+  | `(    degree %%_ = %%n) :=
+    refine ``((degree_eq_iff_nat_degree_eq_of_pos (by norm_num : 0 < _)).mpr _)
+  | `(nat_degree %%_ = %%_) := do
+    wks ← try_core single_term_suggestions,
+    match wks with
+    | some wor :=
+      if single.is_some then refine wor.2 else (do pwks ← pp wor.1, fail!"Try this: exact {pwks}")
+    | none := skip
+    end
+  | _ := fail "Goal is not of the form\n`f.nat_degree = d` or `f.degree = d`"
+  end;
+  do `(nat_degree %%pol = %%degv) ← target |
+      fail "Goal is not of the form\n`f.nat_degree = d` or `f.degree = d`",
+  deg ← guess_degree' pol,
+  degvn ← eval_expr' ℕ degv,
+  guard (deg = degvn) <|>
+    ( do ppe ← pp deg, ppg ← pp degvn,
+      fail sformat!("'{ppe}' is the expected degree\n'{ppg}' is the given degree\n") ),
+  refine ``(le_antisymm _ (le_nat_degree_of_ne_zero _)),
+  focus' [compute_degree_le, simp_coeff []]
+
+end parsing
+
+/--  `prove_monic` tries to close goals of the form `monic f`.  It converts the
+goal to showing that
+* the degree is at most `d`, calling `compute_degree_le` to solve this goal;
+* the coefficient of degree `d` equals `1`, calling `simp_coeff` to simplify this goal.
+Unless the polynomial is particularly complicated, `prove_monic` will either succeed or leave
+a simpler goal to prove.
+ -/
+meta def prove_monic : tactic unit :=
+focus $ do
+  `(monic %%pol) ← target >>= (λ f, whnf f reducible) | fail"Goal is not of the form `monic f`",
+  deg ← guess_degree' pol,
+  deg ← to_expr deg.to_pexpr tt ff,
+  refine ``(monic_of_nat_degree_le_of_coeff_eq_one %%deg _ _),
+  focus' [compute_degree_le, simp_coeff []],
+  try reflexivity
 
 add_tactic_doc
 { name := "compute_degree_le",
@@ -182,5 +535,4 @@ add_tactic_doc
   tags := ["arithmetic", "finishing"] }
 
 end interactive
-
 end tactic
